\section{Euler-Cauchy Equations}

\begin{enumerate}
    \item Auxiliary equation has a double root,
          \begin{align}
              (1-a)^{2}       & = 4b                                             \\
              y_{2}           & = x^{(1-a)/2}\ln x                               \\
              0               & =               x^{2}y'' +
              axy' + \left[ \frac{(1-a)^{2}}{4} \right]y                         \\
              y_{2}'          & = x^{(-1-a)/2} \left[ 1 +
              \left( \frac{1-a}{2} \right)\ln x  \right]                         \\
              y_{2}''         & = x^{(-3-a)/2}\left[ -a +
              \ln x \left( \frac{a^{2}-1}{4} \right) \right]                     \\
              x^{2}y'' + axy' & = x^{(1-a)/2}\left[\ln x \left( \frac{-a^{2}-1 +
              2a}{4} \right)  \right]                                            \\
                              & = x^{(1-a)/2}\ \ln x\left[ \frac{-(1-a)^{2}}{4}
              \right]                                                            \\
                              & = \left[ \frac{-(1-a)^{2}}{4} \right] y
          \end{align}
          Now, if the roots are distinct,
          \begin{align}
              (1-a)^{2}            & > 4b                                              \\
              y                    & = x^{m_{1}}\ln x                                  \\
              y'                   & = x^{m_{1}-1}(1 + m_{1}\ln x)                     \\
              y''                  & = x^{m_{1} - 2}(2m_{1}-1 + m_{1}(m_{1} - 1)\ln x) \\
              x^{2}y'' + axy' + by & = x^{m_{1}} \Big[ 2m_{1} - 1 + a                  \\
                                   & + \{m_{1}^{2} + (a-1)m_{1} + b\}\ln x \Big]       \\
                                   & = 2x^{m_{1}}\left[ m_{1} - \left( \frac{1-a}{2}
                  \right) \right]
          \end{align}
          Thus, the fact that the roots are distinct makes this not satisfy the ODE.
          If instead, the roots were repeated, $ m = (1-a)/2 $ holds and the ODE
          is satisfied.

    \item Finding the general solution
          \begin{align}
              x^{2}y'' -20y & = 0                        &
              a             & = 0, \quad b= -20            \\
              (a-1)^{2}-4b  & = 81 > 0                   &
              m_{1}, m_{2}  & = -4, 5                      \\
              y             & = c_{1}x^{-4} + c_{2}x^{5}
          \end{align}

    \item Finding the general solution
          \begin{align}
              5x^{2}y'' + 23xy' + 16.2y & = 0                             &
              a                         & = 4.6, \quad b= 3.24              \\
              (a-1)^{2}-4b              & = 0                             &
              m_{1}, m_{2}              & = -1.8                            \\
              y                         & = (c_{1} + c_{2}\ln x )x^{-1.8}
          \end{align}

    \item Finding the general solution
          \begin{align}
              x^{2}y'' + 2xy' & = 0                   &
              a               & = 2, \quad b= 0         \\
              (a-1)^{2}-4b    & = 1 > 0               &
              m_{1}, m_{2}    & = -1, 0                 \\
              y               & = c_{1} + c_{2}x^{-1}
          \end{align}

    \item Finding the general solution
          \begin{align}
              4x^{2}y'' + 5y & = 0                                     &
              a              & = 0, \quad b= 5/4                         \\
              (a-1)^{2}-4b   & = -4 < 0                                &
              m_{1}, m_{2}   & = 0.5 \pm i                               \\
              y              & = e^{0.5x}[A\cos(\ln x) + B\sin(\ln x)]
          \end{align}

    \item Finding the general solution
          \begin{align}
              x^{2}y'' + 0.7xy' - 0.1y & = 0                            &
              a                        & = 0.7, \quad b= -0.1             \\
              (a-1)^{2}-4b             & = 0.49 > 0                     &
              m_{1}, m_{2}             & =  0.5, -0.2                     \\
              y                        & = c_{1}x^{0.5} + c_{2}x^{-0.2}
          \end{align}

    \item Finding the general solution
          \begin{align}
              (x^{2}D^{2} - 4xD + 6I)y & = 0                       &
              a                        & = -4, \quad b= 6            \\
              (a-1)^{2}-4b             & = 1 > 0                   &
              m_{1}, m_{2}             & =  3, 2                     \\
              y                        & = c_{1}x^{3} + c_{2}x^{2}
          \end{align}

    \item Finding the general solution
          \begin{align}
              (x^{2}D^{2} - 3xD + 4I)y & = 0                           &
              a                        & = -3, \quad b= 4                \\
              (a-1)^{2}-4b             & = 0                           &
              m_{1}, m_{2}             & =  2                            \\
              y                        & = [ c_{1} + c_{2}\ln x ]x^{2}
          \end{align}

    \item Finding the general solution
          \begin{align}
              (x^{2}D^{2} - 0.2xD + 0.36I)y & = 0                              &
              a                             & = -0.2, \quad b= 0.36              \\
              (a-1)^{2}-4b                  & = 0                              &
              m_{1}, m_{2}                  & =  0.6                             \\
              y                             & = [ c_{1} + c_{2} \ln x ]x^{0.6}
          \end{align}

    \item Finding the general solution
          \begin{align}
              (x^{2}D^{2} - xD + 5I)y & = 0                                      &
              a                       & = -1, \quad b= 5                           \\
              (a-1)^{2}-4b            & = -16 < 0                                &
              m_{1}, m_{2}            & =  1 \pm 2i                                \\
              y                       & = e^{x}[A\cos(2 \ln x) + B\sin(2 \ln x)]
          \end{align}

    \item Finding the general solution
          \begin{align}
              (x^{2}D^{2} - 3xD + 10I)y & = 0                             &
              a                         & = -3, \quad b= 10                 \\
              (a-1)^{2}-4b              & = -24 < 0                       &
              m_{1}, m_{2}              & =  2 \pm \sqrt{6}i                \\
              y                         & = x^{2} [A\cos(\sqrt{6}\ln x) +
                      B\sin(\sqrt{6}\ln x)]
          \end{align}

    \item Solving the IVP $ y(1) = 0.4,\ y'(1) = 0 $ and graphing,
          \begin{align}
              x^{2}y'' - 4xy' + 6y & = 0                       &
              a                    & = -4, \quad b= 6            \\
              (a-1)^{2}-4b         & = 1 > 0                   &
              m_{1}, m_{2}         & =  3, 2                     \\
              y                    & = c_{1}x^{3} + c_{2}x^{2}   \\
              y(1)                 & = c_{1} + c_{2} = 0.4     &
              y'(1)                & = 3c_{1} + 2c_{2} = 0       \\
              c_{1}                & = -0.8                    &
              c_{2}                & = 1.2
          \end{align}
          \begin{figure}[H]
              \centering
              \begin{tikzpicture}
                  \begin{axis}[
                          %   ymode = log,
                          %   axis equal,
                          %   restrict y to domain = -5:20,
                          legend pos = north east,
                          grid = both,
                          width = 12cm,
                          height = 8cm,
                          Ani,
                      ]
                      \addplot[GraphSmooth, y_h, domain=-4:4,]
                      {-0.8*x^(3) + 1.2*x^(2)};
                      \node[GraphNode, label={45:(1, 0.4)}] at (axis cs:1, 0.4) {};
                      \addlegendentry{$y = -0.8x^{3} + 1.2x^{2}$};
                  \end{axis}
              \end{tikzpicture}
          \end{figure}

    \item Solving the IVP $ y(1) = 1,\ y'(1) = -1.5 $ and graphing,
          \begin{align}
              x^{2}y'' + 3xy' + 0.75y & = 0                             &
              a                       & = 3, \quad b= 0.75                \\
              (a-1)^{2}-4b            & = 1 > 0                         &
              m_{1}, m_{2}            & =  -1.5, -0.5                     \\
              y                       & = c_{1}x^{-1.5} + c_{2}x^{-0.5}   \\
              y(1)                    & = c_{1} + c_{2} = 1             &
              y'(1)                   & = -1.5c_{1} - 0.5c_{2} = -1.5     \\
              c_{1}                   & = 1                             &
              c_{2}                   & = 0
          \end{align}
          \begin{figure}[H]
              \centering
              \begin{tikzpicture}
                  \begin{axis}[
                          %   ymode = log,
                          %   axis equal,
                          restrict y to domain = 0:10,
                          legend pos = north east,
                          grid = both,
                          width = 12cm,
                          height = 8cm,
                          Ani,
                      ]
                      \addplot[GraphSmooth, y_h, domain=0:2,]
                      {*x^(-1.5)};
                      \node[GraphNode, label={45:(1, 1)}] at (axis cs:1, 1) {};
                      \addlegendentry{$y = x^{-1.5}$};
                  \end{axis}
              \end{tikzpicture}
          \end{figure}

    \item Solving the IVP $ y(1) = 0,\ y'(1) = 2.5 $ and graphing,
          \begin{align}
              x^{2}y'' + xy' + 9y & = 0                                       &
              a                   & = 1, \quad b= 9                             \\
              (a-1)^{2}-4b        & = -36 < 0                                 &
              m_{1}, m_{2}        & =  0 \pm 3i                                 \\
              y                   & = c_{1}\cos(3 \ln x) + c_{2}\sin(3 \ln x)   \\
              y(1)                & = c_{1} = 0                                 \\
              y'(1)               & = 3c_{2} = 2.5                            &
              c_{2}               & = \frac{5}{6}
          \end{align}
          \begin{figure}[H]
              \centering
              \begin{tikzpicture}
                  \begin{axis}[
                          xmode = log,
                          %   axis equal,
                          %   restrict y to domain = -100:100,
                          legend pos = north west,
                          grid = both,
                          width = 12cm,
                          height = 8cm,
                          Ani,
                      ]
                      \addplot[GraphSmooth, y_h, domain=0.01:10,]
                      {(5/6)*sin(3*ln(x))};
                      \node[GraphNode, label={135:(1, 0)}] at (axis cs:1, 0) {};
                      \addlegendentry{$y = (5/6)\sin(3\ln x)$};
                  \end{axis}
              \end{tikzpicture}
          \end{figure}

    \item Solving the IVP $ y(1) = 3.6,\ y'(1) = 0.4 $ and graphing,
          \begin{align}
              x^{2}y'' + 3xy' + y & = 0                             \\
              a                   & = 3, \quad b= 1                 \\
              (a-1)^{2}-4b        & = 0                           &
              m_{1}, m_{2}        & =  -1                           \\
              y                   & = (c_{1} + c_{2} \ln x)x^{-1}   \\
              y(1)                & = c_{1} = 3.6                 &
              y'(1)               & = c_{2} - c_{1} = 0.4           \\
              c_{2}               & = 4.0
          \end{align}
          \begin{figure}[H]
              \centering
              \begin{tikzpicture}
                  \begin{axis}[
                          restrict y to domain = -10:10,
                          legend pos = south east,
                          grid = both,
                          width = 12cm,
                          height = 8cm,
                          Ani,
                      ]
                      \addplot[GraphSmooth, y_h, domain=0:10,]
                      {x^(-1)*(3.6 + 4*ln(x))};
                      \node[GraphNode, label={-85:(1, 3.6)}] at (axis cs:1, 3.6) {};
                      \addlegendentry{$y = x^{-1}(3.6 + 4\ln x)$};
                  \end{axis}
              \end{tikzpicture}
          \end{figure}

    \item Solving the IVP $ y(1) = -\pi,\ y'(1) =  2\pi $ and graphing,
          \begin{align}
              (x^{2}D^{2} - 3xD + 4I)y & = 0                           &
              a                        & = -3, \quad b= 4                \\
              (a-1)^{2}-4b             & = 0                           &
              m_{1}, m_{2}             & =  2                            \\
              y                        & = [ c_{1} + c_{2}\ln x ]x^{2}   \\
              y(1)                     & = c_{1} = -\pi                &
              y'(1)                    & = c_{2} + 2c_{1} = 2\pi         \\
              c_{2}                    & = 4\pi
          \end{align}
          \begin{figure}[H]
              \centering
              \begin{tikzpicture}
                  \begin{axis}[
                          %   restrict y to domain = -10:10,
                          legend pos = north west,
                          grid = both,
                          width = 12cm,
                          height = 8cm,
                          Ani,
                      ]
                      \addplot[GraphSmooth, y_h, domain=0:2,]
                      {x^(2)*(-pi + 4*pi*ln(x))};
                      \node[GraphNode, label={90:(1, $-\pi$)}] at (axis cs:1, -pi) {};
                      \addlegendentry{$y = x^{2}(-\pi + 4\pi\ln x)$};
                  \end{axis}
              \end{tikzpicture}
          \end{figure}

    \item Solving the IVP $ y(1) = 1,\ y'(1) = 1 $ and graphing,
          \begin{align}
              (x^{2}D^{2} + xD + I)y & = 0                                   &
              a                      & = 1, \quad b= 1                         \\
              (a-1)^{2}-4b           & = -4 < 0                              &
              m_{1}, m_{2}           & =  0 \pm i                              \\
              y                      & = c_{1}\cos(\ln x) + c_{2}\sin(\ln x)   \\
              y(1)                   & = c_{1} = 1                           &
              y'(1)                  & = c_{2} = 1
          \end{align}
          \begin{figure}[H]
              \centering
              \begin{tikzpicture}
                  \begin{axis}[
                          xmode = log,
                          %   axis equal,
                          %   restrict y to domain = 0:200,
                          legend pos = north east,
                          grid = both,
                          width = 12cm,
                          height = 8cm,
                          Ani,
                      ]
                      \addplot[GraphSmooth, y_h, domain=0.01:10000,]
                      {sin(ln(x)) + cos(ln(x))};
                      \node[GraphNode, label={180:(1, 1)}] at (axis cs:1, 1) {};
                      \addlegendentry{$y = \cos(\ln x) + \sin(\ln x)$};
                  \end{axis}
              \end{tikzpicture}
          \end{figure}

    \item Solving the IVP $ y(1) = 1,\ y'(1) = 0 $ and graphing,
          \begin{align}
              (9x^{2}D^{2} + 3xD + I)y & = 0                            &
              a                        & = 1/3, \quad b= 1/9              \\
              (a-1)^{2}-4b             & = 0                            &
              m_{1}, m_{2}             & =  1/3                           \\
              y                        & = x^{1/3}(c_{1} + c_{2} \ln x)   \\
              y(1)                     & = c_{1} = 1                    &
              y'(1)                    & = \frac{c_{1}}{3} + c_{2} = 0    \\
              c_{2}                    & = -1/3
          \end{align}
          \begin{figure}[H]
              \centering
              \begin{tikzpicture}
                  \begin{axis}[
                          %   axis equal,
                          %   restrict y to domain = 0:200,
                          legend pos = north west,
                          grid = both,
                          width = 12cm,
                          height = 8cm,
                          Ani,
                      ]
                      \addplot[GraphSmooth, y_h, domain=0:1.2,]
                      {x^(1/3)*(1 + (1/3)*ln(x))};
                      \node[GraphNode, label={135:(1, 1)}] at (axis cs:1, 1) {};
                      \addlegendentry{$y = (1 + 1/3 \ln x)x^{1/3}$};
                  \end{axis}
              \end{tikzpicture}
          \end{figure}

    \item Solving the IVP $ y(1) = 0.1,\ y'(1) = -4.5 $ and graphing,
          \begin{align}
              (x^{2}D^{2}  - xD - 15I)y & = 0                        &
              a                         & = -1, \quad b= -15           \\
              (a-1)^{2}-4b              & = 64 > 0                   &
              m_{1}, m_{2}              & =  -3, 5                     \\
              y                         & = c_{1}x^{-3} + c_{2}x^{5}   \\
              y(1)                      & = c_{1} + c_{2} = 0.1      &
              y'(1)                     & = -3c_{1} + 5c_{2} = -4.5    \\
              c_{2}                     & = -0.525                   &
              c_{1}                     & = 0.625
          \end{align}
          \begin{figure}[H]
              \centering
              \begin{tikzpicture}
                  \begin{axis}[
                          %   axis equal,
                          restrict y to domain = -100:100,
                          legend pos = north east,
                          grid = both,
                          width = 12cm,
                          height = 8cm,
                          Ani,
                      ]
                      \addplot[GraphSmooth, y_h, domain=-4:4,]
                      {0.625*x^(-3) - 0.525*x^(5)};
                      \node[GraphNode, label={45:(1, 0.1)}] at (axis cs:1, 0.1) {};
                      \addlegendentry{$y = 0.625x^{-3} - 0.525x^{5}$};
                  \end{axis}
              \end{tikzpicture}
          \end{figure}

    \item \begin{enumerate}
              \item By reduction of order with one solution $y_{1} = x^{(1-a)/2}$, and
                    the auxiliary equation having repeated roots.
                    \begin{align}
                        0              & = m^{2} + (a-1)m + by                     \\
                        b              & = \frac{(1-a)^{2}}{4}                     \\
                        0              & = x^{2}y'' + axy' + \frac{(1-a)^{2}}{4}y  \\
                        y_{2} = uy_{1} & = ux^{(1-a)/2}                            \\
                        y_{2}'         & = u'x^{(1-a)/2}
                        + \frac{u(1-a)}{2}x^{(-1-a)/2}                             \\
                        y_{2}''        & = u''x^{(1-a)/2}
                        + u'(1-a)x^{(-1-a)/2} + \frac{u(a^{2} - 1)}{4}x^{(-3-a)/2} \\
                        0              & = u''x^{(5-a)/2}
                        + u'(1-a)x^{(3-a)/2} + \frac{u(a^{2} - 1)}{4}x^{(1-a)/2}   \\
                                       & + au'x^{(3-a)/2}
                        + \frac{au(1-a)}{2}x^{(1-a)/2}  + \frac{u(1-a)^{2}}{4}
                        x^{(1-a)/2}                                                \\
                        0              & = u'' x^{(5-a)/2}
                        + u' x^{(3-a)/2} = u''x + u'                               \\
                        z              & = u' \qquad z' = u''                      \\
                        z'             & = \frac{-z}{x}  \qquad \implies z
                        = \frac{1}{x} \qquad \implies u = \ln x                    \\
                        y_{2}          & = y_{1}\ln x
                    \end{align}

              \item Let $ y_{1} = x^{m} $ and $ y_{2} = x^{m+s} $,
                    \begin{align}
                        0                   & = y'' + (1 -2m - s)y' + (m^{2} + ms)y \\
                        y_{3}               & = \frac{x^{m+s} - x^{m}}{(m+s) - s}
                        = \frac{x^{m+s} - x^{m}}{s}                                 \\
                        \lim_{s \to 0}y_{3} & = \lim_{s \to 0} \diff*{x^{m+s}}{s}
                        \cdot \frac{1}{\difs ss}                                    \\
                                            & = \lim_{s \to 0} x^{m}\diff*{\exp(s
                        \ \ln x)}{s}                                                \\
                                            & = \lim_{s \to 0} x^{m}\left( x^{s}
                        \ln x \right) = x^{m}\ln x
                    \end{align}

              \item In the critical case, with repeated roots $ b = (1-a)^{2}/4 $,
                    \begin{align}
                        0                    & = x^{2}y'' + axy' + by            \\
                        y_{2}                & = x^{(1-a)/2}\ln x                \\
                        y_{2}'               & = x^{(-1-a)/2} \left[ 1
                        + \left( \frac{1-a}{2} \right)\ln x \right]              \\
                        y_{2}''              & = x^{(-3-a)/2} \left[ -a
                        + \left( \frac{a^{2} - 1}{4} \right) \ln x \right]       \\
                        x^{2}y'' + axy' + by & = x^{(1-a)/2} \left[  \frac{a^{2}
                        - 1 + 2a - 2a^{2} + (1-a)^{2}}{4} \right] \ln x          \\
                                             & = 0
                    \end{align}
                    Thus, $ x^{(1-a)/2}\ln x $ is indeed a solution to the ODE when
                    the auxiliary equation has repeated roots.

              \item Substitute $ x = e^{t} \qquad (x>0)$,
                    \begin{align}
                        x^{2}y'' + axy' + by      & = 0                                \\
                        y'                        & = \frac{\difs yt}{\difs xt}
                        = e^{-t}\diff yt                                               \\
                        y''                       & = \diff* {\left( e^{-t}\diff
                            yt \right)}{x} = \frac{1}{\difs xt}\ \diff* {\left( e^{-t}
                        \diff yt \right)}{t}                                           \\
                                                  & = e^{-2t}\left(\diff[2] yt
                        - \diff yt  \right)                                            \\
                        e^{2t}y'' + ae^{t}y' + by & = \diff[2] yt + (a-1)\diff yt + by
                    \end{align}

              \item Let $y_{1}, y_{2} = e^{\lambda_{1} t}, e^{\lambda_{2} t}$ be
                    solutions to the above ODE in $ y, t $, with
                    $ \lambda_{2} = \lambda_{1} + \delta $
                    \begin{align}
                        \lambda^{2} + (a-1)\lambda + b
                                                 & = 0                       \\
                        b                        & = (a - 1)^{2} / 4         \\
                        \text{By superposition} \quad y_{3}
                                                 & = \frac{e^{\lambda_{2} t}
                        - e^{\lambda_{1} t}}{\lambda_{2} - \lambda_{1}}      \\
                        \lim_{\delta \to 0}y_{3} & = \lim_{\delta \to 0}
                        \diff {y_{3}}{\delta}                                \\
                                                 & =\lim_{\delta \to 0}
                        \diff*{\frac{e^{\lambda_{1}t}(e^{\delta t} - 1)}{\delta}}
                        {\delta}                                             \\
                                                 & = \lim_{\delta \to 0}
                        t e^{\lambda_{1}t}e^{\delta t} = te^{\lambda_{1}t}
                    \end{align}
                    The two solutions are $ e^{\lambda t} $ and $ te^{\lambda t} $,
                    which when converted back to functions of $ x $, become
                    $ x^{\lambda} $ and $ x^{\lambda} \ln x $.
          \end{enumerate}
\end{enumerate}