\section{Solution by Variation of Parameters}

\begin{enumerate}
    \item Solving the h-ODE,
          \begin{align}
              y'' + 9y                 & = 0                          &
              a                        & = 0 \qquad b = 9               \\
              \lambda_{1}, \lambda_{2} & = \frac{0 \pm i\sqrt{36}}{2} &
                                       & = 0 \pm 3i                     \\
              y_{h}                    & = {\color{y_h} c_{1}\cos(3x)
              + c_{2}\sin(3x)}
          \end{align}
          Solving the nh-ODE by variation of parameters,
          \begin{align}
              r(x)            & = \sec(3x)                                        \\
              W(y_{1}, y_{2}) & = 3\cos^{2}(3x) + 3\sin^{2}(3x) = 3               \\
              f'              & = \frac{-y_{2}r}{W} = \frac{-\tan(3x)}{3}       &
              g'              & = \frac{y_{1}r}{W} = \frac{1}{3}                  \\
              f               & = \frac{1}{9}\ln|\cos(3x)|                      &
              g               & = \frac{x}{3}                                     \\
              y_{p}           & = {\color{y_p} \frac{\ln|\cos(3x)|}{9} \cos(3x)
              + \frac{x}{3}\sin(3x)}                                              \\
              y               & = {\color{y_h} y_{h}} + {\color{y_p} y_{p}}
          \end{align}

    \item Solving the h-ODE,
          \begin{align}
              y'' + 9y                 & = 0                          &
              a                        & = 0 \qquad b = 9               \\
              \lambda_{1}, \lambda_{2} & = \frac{0 \pm i\sqrt{36}}{2} &
                                       & = 0 \pm 3i                     \\
              y_{h}                    & = {\color{y_h} c_{1}\cos(3x)
              + c_{2}\sin(3x)}
          \end{align}
          Solving the nh-ODE by variation of parameters,
          \begin{align}
              r(x)            & = \csc(3x)                                    \\
              W(y_{1}, y_{2}) & = 3\cos^{2}(3x) + 3\sin^{2}(3x) = 3           \\
              f'              & = \frac{-y_{2}r}{W} = \frac{-1}{3}          &
              g'              & = \frac{y_{1}r}{W} = \frac{\cot(3x)}{3}       \\
              f               & = \frac{-x}{3}                              &
              g               & = \frac{\ln|\sin(3x)|}{9}                     \\
              y_{p}           & = {\color{y_p} \frac{-x}{3} \cos(3x)
              + \frac{\ln|\sin(3x)|}{9}\sin(3x)}                              \\
              y               & = {\color{y_h} y_{h}} + {\color{y_p} y_{p}}
          \end{align}

    \item Solving the h-ODE,
          \begin{align}
              x^{2}y'' - 2xy' + 2y     & = 0                                 &
              a - 1                    & = -3 \qquad b = 2                     \\
              \lambda_{1}, \lambda_{2} & = \frac{3 \pm \sqrt{1}}{2}          &
                                       & = 2, 1                                \\
              y_{h}                    & = {\color{y_h} c_{1}x + c_{2}x^{2}}
          \end{align}
          Solving the nh-ODE by variation of parameters,
          \begin{align}
              r(x)            & = x\sin(x)                                    \\
              W(y_{1}, y_{2}) & = 2x^{2} - x^{2} = x^{2}                      \\
              f'              & = \frac{-y_{2}r}{W} = -x\sin(x)             &
              g'              & = \frac{y_{1}r}{W} = \sin(x)                  \\
              f               & = x\cos(x) - \sin(x)                        &
              g               & = -\cos(x)                                    \\
              y_{p}           & = {\color{y_p} -x\sin(x)}                     \\
              y               & = {\color{y_h} y_{h}} + {\color{y_p} y_{p}}
          \end{align}

    \item Solving the h-ODE,
          \begin{align}
              y'' - 4y' + 5y           & = 0                          &
              a                        & = -4 \qquad b = 5              \\
              \lambda_{1}, \lambda_{2} & = \frac{4 \pm i\sqrt{4}}{2}  &
                                       & = 2 \pm i                      \\
              y_{h}                    & = {\color{y_h} [c_{1}\cos(x)
                  + c_{2}\sin(x)]e^{2x}}
          \end{align}
          Solving the nh-ODE by variation of parameters,
          \begin{align}
              r(x)            & = e^{2x}\csc x                                \\
              W(y_{1}, y_{2}) & = e^{4x}\cos(x)[\cos x + 2\sin x]             \\
                              & - e^{4x}\sin x[-\sin x + 2\cos x]             \\
                              & = e^{4x}                                      \\
              f'              & = \frac{-y_{2}r}{W} = -1                    &
              g'              & = \frac{y_{1}r}{W} = \cot x                   \\
              f               & = -x                                        &
              g               & = \ln|\sin(x)|                                \\
              y_{p}           & = {\color{y_p} e^{2x}[-x\cos x
              + \ln\left( |\sin x| \right) \sin x]}                           \\
              y               & = {\color{y_h} y_{h}} + {\color{y_p} y_{p}}
          \end{align}

    \item Solving the h-ODE,
          \begin{align}
              y'' + y                  & = 0                                         &
              a                        & = 0 \qquad b = 1                              \\
              \lambda_{1}, \lambda_{2} & = \frac{0 \pm i\sqrt{4}}{2}                 &
                                       & = 0 \pm i                                     \\
              y_{h}                    & = {\color{y_h} c_{1}\cos(x) + c_{2}\sin(x)}
          \end{align}
          Solving the nh-ODE by undetermined coefficients,
          \begin{align}
              y'' + y      & = \cos x - \sin x                              \\
              y_{p}        & = Kx\cos x + Mx\sin x                          \\
              y_{p}'       & = \cos x [K + Mx] + \sin x [M - Kx]            \\
              y_{p}''      & = \cos x [2M - Kx] + \sin x [-2K - Mx]         \\
              1            & = 2M                                         &
              \cdots\cdots & [\cos x]                                       \\
              -1           & =  -2K                                       &
              \cdots\cdots & [\sin x]                                       \\
              y_{p}        & = {\color{y_p} \frac{x}{2}[\cos x + \sin x]}   \\
              y            & = {\color{y_h} y_{h}} + {\color{y_p} y_{p}}
          \end{align}

    \item Solving the h-ODE,
          \begin{align}
              y'' + 6y' + 9y           & = 0                                     &
              a                        & = 6 \qquad b = 9                          \\
              \lambda_{1}, \lambda_{2} & = \frac{-6 \pm i\sqrt{0}}{2}            &
                                       & = -3, -3                                  \\
              y_{h}                    & = {\color{y_h} (c_{1} + c_{2}x)e^{-3x}}
          \end{align}
          Solving the nh-ODE by variation of parameters,
          \begin{align}
              r(x)            & = \frac{16}{x^{2} + 1}\ e^{-3x}                \\
              W(y_{1}, y_{2}) & = e^{-6x}                                      \\
              f'              & = \frac{-y_{2}r}{W} = \frac{-16x}{1 + x^{2}} &
              g'              & = \frac{y_{1}r}{W} = \frac{16}{1 + x^{2}}      \\
              f               & = -8\ln(1 + x^{2})                           &
              g               & = 16\arctan x                                  \\
              y_{p}           & = {\color{y_p} e^{-3x}[-8\ln(1 + x^{2})
              + 16x \arctan x]}                                                \\
              y               & = {\color{y_h} y_{h}} + {\color{y_p} y_{p}}
          \end{align}

    \item Solving the h-ODE,
          \begin{align}
              y'' - 4y' + 4y           & = 0                                    &
              a                        & = -4 \qquad b = 4                        \\
              \lambda_{1}, \lambda_{2} & = \frac{4 \pm i\sqrt{0}}{2}            &
                                       & = 2, 2                                   \\
              y_{h}                    & = {\color{y_h} (c_{1} + c_{2}x)e^{2x}}
          \end{align}
          Solving the nh-ODE by variation of parameters,
          \begin{align}
              r(x)            & = 6e^{2x}x^{-4}                               \\
              W(y_{1}, y_{2}) & = e^{4x}                                      \\
              f'              & = \frac{-y_{2}r}{W} = -6x^{-3}              &
              g'              & = \frac{y_{1}r}{W} = 6x^{-4}                  \\
              f               & = 3x^{-2}                                   &
              g               & = -2x^{-3}                                    \\
              y_{p}           & = {\color{y_p} e^{2x}[x^{-2}]}                \\
              y               & = {\color{y_h} y_{h}} + {\color{y_p} y_{p}}
          \end{align}

    \item Solving the h-ODE,
          \begin{align}
              y'' + 4y                 & = 0                          &
              a                        & = 0 \qquad b = 4               \\
              \lambda_{1}, \lambda_{2} & = \frac{0 \pm i\sqrt{16}}{2} &
                                       & = 0 \pm 2i                     \\
              y_{h}                    & = {\color{y_h} c_{1}\cos(2x)
              + c_{2}\sin(2x)}
          \end{align}
          Solving the nh-ODE by undetermined coefficients,
          \begin{align}
              y'' + 4y     & = \cosh(2x) = 0.5e^{2x} + 0.5e^{-2x}          \\
              y_{p}        & = K\cosh(2x)                                  \\
              1            & =  4K + 4K                                  &
              \cdots\cdots & [\cosh(2x)]                                   \\
              y_{p}        & = {\color{y_p} \frac{1}{8}\cosh(2x)}          \\
              y            & = {\color{y_h} y_{h}} + {\color{y_p} y_{p}}
          \end{align}

    \item Solving the h-ODE,
          \begin{align}
              y'' - 2y' + 1y           & = 0                                   &
              a                        & = -2 \qquad b = 1                       \\
              \lambda_{1}, \lambda_{2} & = \frac{2 \pm i\sqrt{0}}{2}           &
                                       & = 1, 1                                  \\
              y_{h}                    & = {\color{y_h} (c_{1} + c_{2}x)e^{x}}
          \end{align}
          Solving the nh-ODE by variation of parameters,
          \begin{align}
              r(x)            & = 35e^{x}x^{1.5}                              \\
              W(y_{1}, y_{2}) & = e^{2x}                                      \\
              f'              & = \frac{-y_{2}r}{W} = -35x^{2.5}            &
              g'              & = \frac{y_{1}r}{W} = 35x^{1.5}                \\
              f               & = -10x^{3.5}                                &
              g               & = 14x^{2.5}                                   \\
              y_{p}           & = {\color{y_p} 4e^{x}x^{3.5}}                 \\
              y               & = {\color{y_h} y_{h}} + {\color{y_p} y_{p}}
          \end{align}

    \item Solving the h-ODE,
          \begin{align}
              y''  + 2y' + 2y          & = 0                          &
              a                        & = 2 \qquad b = 2               \\
              \lambda_{1}, \lambda_{2} & = \frac{-2 \pm i\sqrt{4}}{2} &
                                       & = -1 \pm i                     \\
              y_{h}                    & = {\color{y_h} [c_{1}\cos x
                  + c_{2}\sin x]e^{-x}}
          \end{align}
          Solving the nh-ODE by variation of parameters,
          \begin{align}
              r(x)            & = 4e^{-x}\sec ^{3}x                           \\
              W(y_{1}, y_{2}) & = e^{-2x}                                     \\
              f'              & = \frac{-y_{2}r}{W} = -4\tan x \sec^{2}x    &
              g'              & = \frac{y_{1}r}{W} = 4 \sec^{2}x              \\
              f               & = -2\tan^{2}x                               &
              g               & = 4\tan x                                     \\
              y_{p}           & = {\color{y_p} e^{-x}\sin x\ [2\tan x]}       \\
              y               & = {\color{y_h} y_{h}} + {\color{y_p} y_{p}}
          \end{align}

    \item Solving the h-ODE,
          \begin{align}
              x^{2}y'' - 4xy' + 6y     & = 0                                     &
              a - 1                    & = -5 \qquad b = 6                         \\
              \lambda_{1}, \lambda_{2} & = \frac{5 \pm \sqrt{1}}{2}              &
                                       & = 2, 3                                    \\
              y_{h}                    & = {\color{y_h} c_{1}x^{2} + c_{2}x^{3}}
          \end{align}
          Solving the nh-ODE by variation of parameters,
          \begin{align}
              r(x)            & = 21x^{-6}                                    \\
              W(y_{1}, y_{2}) & = x^{4}                                       \\
              f'              & = \frac{-y_{2}r}{W} = -21x^{-7}             &
              g'              & = \frac{y_{1}r}{W} = 21x^{-8}                 \\
              f               & = \frac{21}{6}x^{-6}                        &
              g               & = -3x^{-7}                                    \\
              y_{p}           & = {\color{y_p} 0.5x^{-4}}                     \\
              y               & = {\color{y_h} y_{h}} + {\color{y_p} y_{p}}
          \end{align}

    \item Solving the h-ODE,
          \begin{align}
              y'' - y                  & = 0                                      &
              a                        & = 0 \qquad b = -1                          \\
              \lambda_{1}, \lambda_{2} & = \frac{0 \pm \sqrt{4}}{2}               &
                                       & = -1, 1                                    \\
              y_{h}                    & = {\color{y_h} c_{1}e^{-x} + c_{2}e^{x}}
          \end{align}
          Solving the nh-ODE by variation of parameters,
          \begin{align}
              r(x)            & = \frac{1}{\cosh x}                                \\
              W(y_{1}, y_{2}) & = 2                                                \\
              f'              & = \frac{-y_{2}r}{W} = \frac{-e^{2x}}{1 + e^{2x}} &
              g'              & = \frac{y_{1}r}{W} = \frac{e^{-2x}}{e^{-2x} + 1}   \\
              f               & = -0.5\ln (1 + e^{2x})                           &
              g               & = -0.5\ln(1 + e^{-2x})                             \\
              y_{p}           & = {\color{y_p} -0.5[e^{-x}\ln(1 + e^{2x})
              + e^{x}\ln(1 + e^{-2x})]}                                            \\
              y               & = {\color{y_h} y_{h}} + {\color{y_p} y_{p}}
          \end{align}

    \item Solving the h-ODE,
          \begin{align}
              x^{2}y'' + xy' - 9y      & = 0                                      &
              a - 1                    & = 0 \qquad b = -9                          \\
              \lambda_{1}, \lambda_{2} & = \frac{0 \pm \sqrt{36}}{2}              &
                                       & = -3, 3                                    \\
              y_{h}                    & = {\color{y_h} c_{1}x^{-3} + c_{2}x^{3}}
          \end{align}
          Solving the nh-ODE by variation of parameters,
          \begin{align}
              r(x)            & = 48x^{3}                                     \\
              W(y_{1}, y_{2}) & = 6x^{-1}                                     \\
              f'              & = \frac{-y_{2}r}{W} = -8x^{7}               &
              g'              & = \frac{y_{1}r}{W} = 8x                       \\
              f               & = -x^{8}                                    &
              g               & = 4x^{2}                                      \\
              y_{p}           & = {\color{y_p} 3x^{5}}                        \\
              y               & = {\color{y_h} y_{h}} + {\color{y_p} y_{p}}
          \end{align}

    \item Applying both methods to compare
          \begin{enumerate}
              \item Solving the h-ODE,
                    \begin{align}
                        y''  + 4y' + 3y          & = 0                         &
                        a                        & = 4 \qquad b = 3              \\
                        \lambda_{1}, \lambda_{2} & = \frac{-4 \pm \sqrt{4}}{2} &
                                                 & = -3, -1                      \\
                        y_{h}                    & = {\color{y_h} c_{1}e^{-3x}
                        + c_{2}e^{-x}}
                    \end{align}
                    Solving the nh-ODE by variation of parameters,
                    \begin{align}
                        r(x)            & = 65\cos(2x)                                \\
                        W(y_{1}, y_{2}) & = 2e^{-4x}                                  \\
                        f'              & = \frac{-y_{2}r}{W} = \frac{-65\cos(2x)
                        e^{3x}}{2}      &
                        g'              & = \frac{y_{1}r}{W} = \frac{65\cos(2x)
                        e^{x}}{2}                                                     \\
                        f               & = \frac{-5e^{3x}}{2}\ [3\cos(2x)
                        + 2\sin(2x)]    &
                        g               & = \frac{13e^{x}}{2} [\cos(2x) + 2\sin(2x)]  \\
                        y_{p}           & = {\color{y_p} -\cos(2x) + 8\sin(2x)}       \\
                        y               & = {\color{y_h} y_{h}} + {\color{y_p} y_{p}}
                    \end{align}

                    Solving the nh-ODE by undetermined coefficients,
                    \begin{align}
                        y'' + 4y' + 3y & = 65\cos(2x)                                  \\
                        y_{p}          & = K\cos(2x) + M\sin(2x)                       \\
                        65             & =  -4K + 8M + 3K                            &
                        \cdots\cdots   & [\cos(2x)]                                    \\
                        0              & =  -4M - 8K + 3M                            &
                        \cdots\cdots   & [\sin(2x)]                                    \\
                        y_{p}          & = {\color{y_p} -\cos(2x) + 8\sin(2x)}         \\
                        y              & = {\color{y_h} y_{h}} + {\color{y_p} y_{p}}
                    \end{align}
                    Both methods match, but method 2 is simpler.

              \item Solving the h-ODE,
                    \begin{align}
                        y''  - 2y' + y           & = 0                        &
                        a                        & = -2 \qquad b = 1            \\
                        \lambda_{1}, \lambda_{2} & = \frac{2 \pm \sqrt{0}}{2} &
                                                 & = 1, 1                       \\
                        y_{h}                    & = {\color{y_h} [c_{1}
                            + c_{2}x]e^{x}}
                    \end{align}
                    Solving the nh-ODE by variation of parameters,
                    \begin{align}
                        r_{1}(x)        & = 35e^{x}x^{1.5}                   \\
                        W(y_{1}, y_{2}) & = e^{2x}                           \\
                        f'              & = \frac{-y_{2}r}{W} = -35x^{2.5} &
                        g'              & = \frac{y_{1}r}{W} = 35x^{1.5}     \\
                        f               & = -10x^{3.5}                     &
                        g               & = 14x^{2.5}                        \\
                        y_{p1}          & = {\color{y_p} 4e^{x}x^{3.5}}
                    \end{align}

                    Solving the nh-ODE by undetermined coefficients,
                    \begin{align}
                        y'' - 2y' + y & = x^{2}                                 \\
                        y_{p2}        & = K_{2}x^{2} + K_{1}x + K_{0}           \\
                        1             & =  K_{2}                              &
                        \cdots\cdots  & [x^{2}]                                 \\
                        0             & =  -4K_{2} + K_{1}                    &
                        \cdots\cdots  & [x]                                     \\
                        0             & =  2K_{2}  - 2K_{1} + K_{0}           &
                        \cdots\cdots  & [1]                                     \\
                        y_{p2}        & = {\color{y_p} x^{2} + 4x + 6}          \\
                        y             & = {\color{y_h} [c_{1} + c_{2}x]e^{x}}
                        + {\color{y_p} 4e^{x}x^{3.5} + x^{2} + 4x + 6}
                    \end{align}
                    Each of the terms in $ r(x) $ are more amenable to one of the
                    methods.

              \item Refer Problem set 2.7, Question 20 for the method of undetermined
                    coefficients applied to Euler-Cauchy ODEs.
          \end{enumerate}
\end{enumerate}