\section{Differentiation and Integration of Transforms, ODEs with Variable Coefficients}
\begin{enumerate}
    \item Refer notes. TBC.

    \item Using differentiation to find the Laplace transform,
          \begin{align}
              g(t) & = \color{y_h} 3t \sinh(4t)             &
              F(s) & = 3\Lap\{\sinh(4t)\}                     \\
              F    & = \frac{12}{s^2 -16}                   &
              G(s) & = -F'(s)                                 \\
              G    & = \color{y_p} \frac{24s}{(s^2 - 16)^2}
          \end{align}

    \item Using differentiation to find the Laplace transform,
          \begin{align}
              g(t) & = \color{y_h} 0.5 t\ e^{-3t}        &
              F(s) & = 0.5 \Lap\{ e^{-3t} \}               \\
              F    & = \frac{0.5}{s + 3}                 &
              G(s) & = -F'(s)                              \\
              G    & = \color{y_p} \frac{0.5}{(s + 3)^2}
          \end{align}

    \item Using differentiation to find the Laplace transform,
          \begin{align}
              g(t) & = \color{y_h} t\ e^{-t}\cos(t)                               &
              F(s) & = \Lap\{ e^{-t}\cos(t) \}                                      \\
              F    & = \frac{(s + 1)}{(s + 1)^2 + 1}                              &
              G(s) & = -F'(s)                                                       \\
              G    & = \frac{(s + 1)(2s + 2) - (s^2 + 2s + 2)}{[(s + 1)^2 + 1]^2} &
              G    & = \color{y_p} \frac{s^2 + 2s}{(s^2 + 2s + 2)^2}
          \end{align}

    \item Using differentiation to find the Laplace transform,
          \begin{align}
              g(t) & = \color{y_h} t\ \cos(\omega t)                         &
              F(s) & = \Lap\{ \cos(\omega t) \}                                \\
              F    & = \frac{s}{s^2 + \omega^2}                              &
              G(s) & = -F'(s)                                                  \\
              G    & = \frac{s(2s) - s^2 - \omega^2}{[s^2 + \omega^2]^2}     &
              G    & = \color{y_p} \frac{s^2 - \omega^2}{(s^2 + \omega^2)^2}
          \end{align}

    \item Using differentiation to find the Laplace transform,
          \begin{align}
              g(t) & = \color{y_h} t^2\ \sin(3t)                            &
              F(s) & = \Lap\{ \sin(3t) \}                                     \\
              F    & = \frac{3}{s^2 + 9}                                    &
              G(s) & = F''(s)                                                 \\
              G    & = \Bigg[ \frac{-6s}{(s^2 + 9)^2} \Bigg]'               &
              G    & = \frac{-6(s^2 + 9)^2 + (24s^2)(s^2 + 9)}{(s^2 + 9)^2}   \\
              G    & = \color{y_p} \frac{18(s^2 - 3)}{(s^2 + 9)^3}
          \end{align}

    \item Using differentiation to find the Laplace transform,
          \begin{align}
              g(t) & = \color{y_h} t^2\ \cosh(2t)                                    &
              F(s) & = \Lap\{ \cosh(2t) \}                                             \\
              F    & = \frac{s}{s^2 - 4}                                             &
              G(s) & = (-1)^2 F''(s)                                                   \\
              G    & = \Bigg[ \frac{-(s^2 + 4)}{(s^2 - 4)^2} \Bigg]'                 &
              G    & = \frac{-(2s)(s^2 - 4)^2 + (4s)(s^2 - 4)(s^2 + 4)}{(s^2 - 4)^4}   \\
              G    & = \color{y_p} \frac{2s^3 + 24s}{(s^2 - 4)^3}
          \end{align}

    \item Using differentiation to find the Laplace transform,
          \begin{align}
              g(t) & = \color{y_h} t\ e^{-kt}\sin(t)                  &
              F(s) & = \Lap\{ e^{-kt}\sin(t) \}                         \\
              F    & = \frac{1}{(s+k)^2 + 1}                          &
              G(s) & = -F'(s)                                           \\
              G    & = \color{y_p} \frac{2(s + k)}{[(s + k)^2 + 1]^2}
          \end{align}

    \item Using differentiation to find the Laplace transform,
          \begin{align}
              g(t) & = \color{y_h} 0.5 t^2\ \sin(\pi t)                      &
              F(s) & = \Lap\{ 0.5 \sin(\pi t) \}                               \\
              F    & = \frac{0.5\pi}{s^2 + \pi^2}                            &
              G(s) & = (-1)^2 F''(s)                                           \\
              G    & = \Bigg[ \frac{-\pi s}{(s^2 + \pi^2)^2} \Bigg]'         &
              G    & = \frac{-\pi(s^2 + \pi^2)^2 + \pi (4s^2) (s^2 + \pi^2)}
              {(s^2 + \pi^2)^4}                                                \\
              G    & = \color{y_p} \frac{\pi (3s^2 - \pi^2)}{(s^2 + \pi)^3}
          \end{align}

    \item Using differentiation to find the Laplace transform,
          \begin{align}
              g(t) & = \color{y_h} t^n\ e^{kt}                       &
              F(s) & = \Lap\{ e^{kt} \}                                \\
              F    & = \frac{1}{s-k}                                 &
              G(s) & = (-1)^n F^{(n)}(s)                               \\
              G    & = \Bigg[ \frac{-\pi s}{(s^2 + \pi^2)^2} \Bigg]' &
              G    & = (-1)^n\ \frac{(-1)^n\ n!}{(s - k)^{n+1}}        \\
              G    & = \color{y_p} \frac{n!}{(s - k)^{n+1}}
          \end{align}

    \item Using differentiation to find the Laplace transform,
          \begin{align}
              g(t) & = \color{y_h} 4t\ \cos(0.5\pi t)                       &
              F(s) & = 4\Lap\{ \cos(0.5 \pi t) \}                             \\
              F    & = \frac{4s}{s^2 + 0.25\pi^2}                           &
              G(s) & = -F'(s)                                                 \\
              G    & = \frac{-4s^2 - \pi^2 + 4s(2s)}{(s^2 + 0.25\pi^2)^2}   &
              G    & = \color{y_p} \frac{4s^2 - \pi^2}{(s^2 + 0.25\pi^2)^2}
          \end{align}

    \item Laguerre's polynomials using explicit algorithm,
          \begin{enumerate}
              \item Using a CAS,
                    \begin{align}
                        l_n    & = \frac{e^t}{n!}\ \difoverride{n}
                        \diff**[n]{t}{(t^n e^{-t})}                                \\
                        l_0    & = 1                                               \\
                        l_1    & = 1 - x                                           \\
                        l_2    & = \frac{x^{2}}{2} - 2 x + 1                       \\
                        l_3    & = - \frac{x^{3}}{6} + \frac{3 x^{2}}{2} - 3 x + 1 \\
                        l_4    & = \frac{x^{4}}{24} - \frac{2 x^{3}}{3} + 3 x^{2}
                        - 4 x + 1                                                  \\
                        l_5    & = - \frac{x^{5}}{120} + \frac{5 x^{4}}{24}
                        - \frac{5 x^{3}}{3} + 5 x^{2} - 5 x + 1                    \\
                        l_6    & = \frac{x^{6}}{720} - \frac{x^{5}}{20}
                        + \frac{5 x^{4}}{8} - \frac{10 x^{3}}{3} + \frac{15 x^{2}}{2}
                        - 6 x + 1                                                  \\
                        l_7    & = - \frac{x^{7}}{5040} + \frac{7 x^{6}}{720}
                        - \frac{7 x^{5}}{40} + \frac{35 x^{4}}{24} - \frac{35 x^{3}}{6}
                        + \frac{21 x^{2}}{2} - 7 x + 1                             \\
                        l_8    & = \frac{x^{8}}{40320} - \frac{x^{7}}{630}
                        + \frac{7 x^{6}}{180} - \frac{7 x^{5}}{15} + \frac{35 x^{4}}{12}
                        - \frac{28 x^{3}}{3} + 14 x^{2} - 8 x + 1                  \\
                        l_9    & = - \frac{x^{9}}{362880} + \frac{x^{8}}{4480}
                        - \frac{x^{7}}{140} + \frac{7 x^{6}}{60} - \frac{21 x^{5}}{20}
                        + \frac{21 x^{4}}{4} - 14 x^{3} + 18 x^{2} - 9 x + 1       \\
                        l_{10} & = \frac{x^{10}}{3628800} - \frac{x^{9}}{36288}
                        + \frac{x^{8}}{896} - \frac{x^{7}}{42} + \frac{7 x^{6}}{24}
                        - \frac{21 x^{5}}{10} + \frac{35 x^{4}}{4} - 20 x^{3}
                        + \frac{45 x^{2}}{2}                                       \\
                               & - 10 x + 1
                    \end{align}
                    The fact that these polynomials satisfy the Laguerre ODE is verified
                    using the CAS (not shown here).
                    \begin{align}
                        ty'' + (1 - t)y' + ny & = 0
                    \end{align}
              \item Using the Laplace transform of the Laguerre polynomials,
                    \begin{align}
                        Y & = \color{y_p} \frac{(s-1)^n}{s^{n+1}}                    &
                        Y & = \sum_{m = 0}^{n} \binom{n}{m} \frac{s^{n-m}\ (-1)^{m}}
                        {s^{n+1}}                                                      \\
                        Y & = \sum_{m = 0}^{n} \binom{n}{m} \frac{(-1)^m}{s^{m+1}}   &
                        y & = \color{y_h} \sum_{m = 0}^{n} \binom{n}{m}
                        \frac{(-1)^m}{m!}\ t^m
                    \end{align}
              \item TBC. Everything on CAS behind the scenes
              \item Given the generating function,
                    \begin{align}
                        \frac{1}{(1 - x)^{p+1}}           & = \sum_{m=0}^{\infty}
                        \frac{(m+p)!}{m!\ p!}\ x^m                                \\
                        \sum_{n = 0}^{\infty} l_n(t)\ x^n & = \frac{1}{(1 - x)}
                        \exp\left( \frac{tx}{x-1} \right)                         \\
                                                          & = \Bigg[
                            \sum_{p=0}^{\infty}\  \frac{(-1)^p}{p!}
                        \frac{t^p\ x^p}{(1 - x)^{p+1}} \Bigg]                     \\
                                                          & = \sum_{p=0}^{\infty}
                        \sum_{m = 0}^{\infty} \frac{(-1)^p\ (m+p)!}{m!\ (p!)^2}
                        \ t^p\ x^{p+m}
                    \end{align}
                    Let $ n = m+p $ in order to collect the coefficients of $ x^n $.
                    THen the coefficient of $ t^p $ is
                    \begin{align}
                        \frac{(-1)^p\ n!}{(p!)^2\ (n-p)!} & = \frac{(-1)^p}{p!}
                        \ \binom{n}{p}
                    \end{align}
                    which aligns with the general term of the Laguerre polynomials in
                    part $ c $ above.
          \end{enumerate}

    \item TBC. Draw graphs.

    \item Finding inverse Laplace transform,
          \begin{align}
              Y(s) & = \color{y_p} \frac{s}{(s^2 + 16)^2}                          \\
              F(s) & = \frac{s}{s^2 + 16}                                        &
              G(s) & = \frac{4}{s^2 + 16}                                          \\
              f(t) & = \cos(4t)                                                  &
              g(t) & = \sin(4t)                                                    \\
              f*g  & = \infint \cos(4r)\ \sin(4t - 4r)\ \dl r                    &
                   & = 0.5 \infint \Big[\sin(4t) + \sin(8r - 4t)\Big]\ \dl r       \\
                   & = \Bigg[ \frac{8r\ \sin(4t) - \cos(8r - 4t)}{16} \Bigg]_0^t &
                   & = \frac{t\ \sin(4t)}{2}                                       \\
              y(t) & = \color{y_h} \frac{t\ \sin(4t)}{8}
          \end{align}

    \item Finding inverse Laplace transform,
          \begin{align}
              Y(s) & = \color{y_p} \frac{s}{(s^2 - 9)^2}                             \\
              F(s) & = \frac{s}{s^2 - 9}                                           &
              G(s) & = \frac{3}{s^2 - 9}                                             \\
              f(t) & = \cosh(3t)                                                   &
              g(t) & = \sinh(3t)                                                     \\
              f*g  & = \infint \cosh(3r)\ \sinh(3t - 3r) \dl r                     &
                   & = 0.5 \infint \Big[\sinh(3t) - \sinh(6r - 3t)\Big] \dl r        \\
                   & = \Bigg[ \frac{6r\ \sinh(3t) - \cosh(6r - 3t)}{12} \Bigg]_0^t &
                   & = \frac{t\ \sinh(3t)}{2}                                        \\
              y(t) & = \color{y_h} \frac{t\ \sinh(3t)}{6}
          \end{align}

    \item Finding inverse Laplace transform,
          \begin{align}
              Y(s) & = \color{y_p} \frac{2(s + 3)}{[(s+3)^2 + 1]^2}   &
              G(s) & = \int_{s}^{\infty} F(p) \dl p                     \\
              G(s) & =  \Bigg[ \frac{-1}{(p+3)^2 + 1} \Bigg]_s^\infty &
              G(s) & = \frac{1}{(s+3)^2 + 1}                            \\
              g(t) & = e^{-3t}\sin(t)                                 &
              f(t) & = \color{y_h} t e^{-3t}\ \sin(t)
          \end{align}

    \item Finding inverse Laplace transform,
          \begin{align}
              Y(s)         & = \color{y_p} \ln\left( \frac{s}{s-1} \right) &
              H(s) = Y'(s) & = \frac{-1}{s(s-1)}                             \\
              F(s)         & = \frac{1}{s}                                 &
              G(s)         & = \frac{1}{(s-1)}                               \\
              f(t)         & = 1                                           &
              g(t)         & = e^{t}                                         \\
              f * g        & = \int_{0}^{t} e^r\ \dl r                     &
              f * g        & = e^t - 1                                       \\
              h(t)         & = 1 - e^t                                     &
              y(t)         & = \color{y_h} \frac{e^t - 1}{t}
          \end{align}

    \item Finding inverse Laplace transform,
          \begin{align}
              Y(s)         & = \color{y_p} \arccot \Bigg(\frac{s}{\pi}\Bigg) &
              H(s) = Y'(s) & = \frac{1}{\pi}\ \frac{-\pi^2}{\pi^2 + s^2}       \\
              h(t)         & = -\sin(\pi t)                                  &
              y(t)         & = \color{y_h} \frac{\sin(\pi t)}{t}
          \end{align}

    \item Finding inverse Laplace transform,
          \begin{align}
              Y(s)               & = \color{y_p} \ln \Bigg[\frac{s^2 + 1}
              {(s - 1)^2} \Bigg] &
              H(s) = Y'(s)       & = \frac{2s}{s^2 + 1} - \frac{2}{s - 1}    \\
              h(t)               & = 2\cos(t) - 2e^t                       &
              y(t)               & = \color{y_h} \frac{2e^t - 2\cos(t)}{t}
          \end{align}

    \item Finding inverse Laplace transform,
          \begin{align}
              Y(s)           & = \color{y_p} \ln \Bigg[\frac{s + a}
              {s + b} \Bigg] &
              H(s) = Y'(s)   & = \frac{1}{s + a} - \frac{1}{s + b}         \\
              h(t)           & = e^{-at} - e^{-bt}                       &
              y(t)           & = \color{y_h} \frac{e^{-bt} - e^{-at}}{t}
          \end{align}

\end{enumerate}