\section{Homogeneous Linear ODEs with Constant Coefficients}
\begin{enumerate}
    \item Solving h-ODE
          \begin{align}
              y''' + 25y'             & = 0                                  \\
              \lambda^{3} + 25\lambda & = 0                                  \\
              \lambda                 & = \{0, 5i, -5i\}                     \\
              y_{h}                   & = {\color{y_h} c_{1} + c_{2}\cos(5x)
              + c_{3}\sin(5x)}
          \end{align}
    \item Solving h-ODE
          \begin{align}
              y^{(iv)} + 2y'' + y            & = 0                             \\
              \lambda^{4} + 2\lambda^{2} + 1 & = 0                             \\
              \lambda                        & = \{i, i, -i, -i\}              \\
              y_{h}                          & = {\color{y_h} [c_{1} + c_{2}x]
              \cos x + [c_{3} + c_{4}x] \sin x}
          \end{align}
    \item Solving h-ODE
          \begin{align}
              y^{(iv)} + 4y''            & = 0                               \\
              \lambda^{4} + 4\lambda^{2} & = 0                               \\
              \lambda                    & = \{0, 0, 2i, -2i\}               \\
              y_{h}                      & = {\color{y_h} [c_{1} + c_{2}x] +
              c_{3}\cos(2x) + c_{4} \sin(2x)}
          \end{align}
    \item Solving h-ODE
          \begin{align}
              y''' - y'' - y' + y                     & = 0                   \\
              \lambda^{3} - \lambda^{2} - \lambda + 1 & = 0                   \\
              \lambda                                 & = \{-1, 1, 1\}        \\
              y_{h}                                   & = {\color{y_h} [c_{1}
                  + c_{2}x]e^{x} +
              c_{3}e^{-x}}
          \end{align}
    \item Solving h-ODE
          \begin{align}
              y^{iv} + 10y'' + 9y             & = 0                        \\
              \lambda^{4} + 10\lambda^{2} + 9 & = 0                        \\
              \lambda                         & = \{-i, i, -3i, 3i\}       \\
              y_{h}                           & = {\color{y_h} c_{1}\cos x
              + c_{2} \sin x + c_{3}\cos(3x) + c_{4}\sin(3x) }
          \end{align}
    \item Solving h-ODE
          \begin{align}
              y^{v} + 8y''' + 16y'                   & = 0                       \\
              \lambda^{5} + 8\lambda^{3} + 16\lambda & = 0                       \\
              \lambda                                & = \{0, 2i, 2i, -2i, -2i\} \\
              y_{h}                                  & = {\color{y_h} [c_{1}
                  + c_{2}x]\cos(2x) +
              [c_{3} + c_{4}x]\sin(x) + c_{5} }
          \end{align}
    \item Solving the h-ODE,
          \begin{align}
              y''' + 3.2y'' + 4.81y'                     & = 0           \\
              \lambda^{3} + 3.2\lambda^{2} + 4.81\lambda & = 0           \\
              \lambda_{1}, \lambda_{2}                   & = \frac{-3.2
              \pm i\sqrt{9}}{2} = -1.6 \pm 1.5i                          \\
              y_{h}                                      & = \color{y_h}
              e^{-1.6x}[c_{1}\cos(1.5x)
                      + c_{2}\sin(1.5x)] + c_{3}
          \end{align}
          Applying IC $ y(0) = 3.4, y'(0) = -4.6, y''(0) = 9.91 $,
          \begin{align}
              3.4   & = c_{1} + c_{3}                                         \\
              -4.6  & = -1.6c_{1} + 1.5c_{2}                                  \\
              9.91  & = 0.31c_{1} - 4.8c_{2}                                  \\
              y_{h} & = \color{y_h} e^{-1.6x}[\cos(1.5x) - 2\sin(1.5x)] + 2.4
          \end{align}
          \begin{figure}[H]
              \centering
              \begin{tikzpicture}[
                      declare function = {
                              y_p = 2.4 + e^(-1.6*x)*(cos(1.5*x) + sin(1.5*x)) ;
                          }
                  ]
                  \begin{axis}[
                          PiStyleX,
                          xtick distance = 0.5*pi,
                          domain = 0:2*pi,
                          legend pos = north east,
                          grid = both,
                          Ani,
                      ]
                      \addplot[GraphSmooth, y_p]{y_p};
                      \addlegendentry{$y_{p}$};
                  \end{axis}
              \end{tikzpicture}
          \end{figure}

    \item Solving the h-ODE,
          \begin{align}
              0               & = y''' + 7.5y'' + 14.25y' - 9.125y                    \\
              0               & = \lambda^{3} + 7.5\lambda^{2} + 14.25\lambda - 9.125 \\
              \{\lambda_{i}\} & = \{0.5, -4 \pm 1.5i\}                                \\
              y_{h}           & = \color{y_h} c_{1}e^{0.5x} +
              + e^{-4x}[c_{2}\cos(1.5x) + c_{3}\sin(1.5x)]
          \end{align}
          Applying IC $ y(0) = 10.05, y'(0) = -54.975, y''(0) = 257.5125 $,
          \begin{align}
              10.05    & = c_{1} + c_{2}                                      \\
              -54.975  & = 0.5c_{1} + 1.5c_{3} - 4c_{2}                       \\
              257.5125 & = 0.25c_{1} + 13.75c_{2} - 14c_{3}                   \\
              y_{h}    & = \color{y_h} -0.65e^{0.5x} + e^{-4x}[10.7\cos(1.5x)
                      - 7.89\sin(1.5x)]
          \end{align}
          \begin{figure}[H]
              \centering
              \begin{tikzpicture}[
                      declare function = {
                              y_p = -0.65*e^(0.5*x) + e^(-4*x)*(10.7*cos(1.5*x)
                              - 7.78*sin(1.5*x)) ;
                          }
                  ]
                  \begin{axis}[
                          PiStyleX,
                          xtick distance = 0.5*pi,
                          domain = 0:2*pi,
                          legend pos = north east,
                          grid = both,
                          Ani,
                      ]
                      \addplot[GraphSmooth, y_p]{y_p};
                      \addlegendentry{$y_{p}$};
                  \end{axis}
              \end{tikzpicture}
          \end{figure}

    \item Solving the h-ODE,
          \begin{align}
              0               & = 4y''' + 8y'' + 41y' + 37y                    \\
              0               & = 4\lambda^{3} + 8\lambda^{2} + 41\lambda + 37 \\
              \{\lambda_{i}\} & = \{-1, -0.5 \pm 3i\}                          \\
              y_{h}           & = \color{y_h} c_{1}e^{-x}
              + e^{-0.5x}[c_{2}\cos(3x) + c_{3}\sin(3x)]
          \end{align}
          Applying IC $ y(0) = 9, y'(0) = -6.5, y''(0) = -39.75 $,
          \begin{align}
              9      & = c_{1} + c_{2}                                 \\
              -6.5   & = -c_{1} - 0.5c_{2} + 3c_{3}                    \\
              -39.75 & = c_{1} - 8.75c_{2} - 3c_{3}                    \\
              y_{h}  & = \color{y_h} 4e^{-x} + e^{-0.5x} [5\cos(1.5x)]
          \end{align}
          \begin{figure}[H]
              \centering
              \begin{tikzpicture}[
                      declare function = {
                              y_p = 4*e^(-x) + e^(-0.5*x)*(5*cos(1.5*x)) ;
                          }
                  ]
                  \begin{axis}[
                          PiStyleX,
                          xtick distance = pi,
                          domain = 0:4*pi,
                          legend pos = north east,
                          grid = both,
                          Ani,
                      ]
                      \addplot[GraphSmooth, y_p]{y_p};
                      \addlegendentry{$y_{p}$};
                  \end{axis}
              \end{tikzpicture}
          \end{figure}

    \item Solving the h-ODE,
          \begin{align}
              0               & = y^{iv} + 4y                                  \\
              0               & = \lambda^{4} + 4                              \\
              \{\lambda_{i}\} & = \{-1 \pm i, 1 \pm i\}                        \\
              y_{h}           & = \color{y_h} e^{x}[c_{1}\cos x + c_{2}\sin x]
              + e^{-x}[c_{3}\cos x + c_{4}\sin x]
          \end{align}
          Applying IC $ y(0) = 1/2, y'(0) = -3/2, y''(0) = 5/2, y'''(0) = -7/2 $,
          \begin{align}
              1/2   & = c_{1} + c_{2}                                    \\
              -3/2  & = c_{1} + c_{2} - c_{3} + c_{4}                    \\
              5/2   & = 2c_{2} - 2c_{4}                                  \\
              -7/2  & = -2c_{1} + 2c_{2} + 2c_{3} + 2c_{4}               \\
              y_{h} & = \color{y_h} \frac{e^{x}}{16}[11\cos x - 3\sin x]
              + \frac{e^{-x}}{16}[9\cos x - 23\sin x]
          \end{align}
          \begin{figure}[H]
              \centering
              \begin{tikzpicture}[
                      declare function = {
                              y_p = (e^(x)/16)*(11*cos(x) - 3*sin(x)) +
                              (e^(-x)/16)*(9*cos(x) - 23*sin(x)) ;
                          }
                  ]
                  \begin{axis}[
                          PiStyleX,
                          xtick distance = 0.4*pi,
                          domain = 0:1.6*pi,
                          legend pos = north west,
                          grid = both,
                          Ani,
                      ]
                      \addplot[GraphSmooth, y_p]{y_p};
                      \addlegendentry{$y_{p}$};
                  \end{axis}
              \end{tikzpicture}
          \end{figure}

    \item Solving the h-ODE,
          \begin{align}
              0               & = y^{iv} - 9y'' - 400y                      \\
              0               & = \lambda^{4} - 9\lambda^{2} - 400          \\
              \{\lambda_{i}\} & = \{-5, 5, -4i, 4i\}                        \\
              y_{h}           & = \color{y_h} c_{1}\cos(4x) + c_{2}\sin(4x)
              + c_{3}e^{-5x} + c_{4}e^{5x}
          \end{align}
          Applying IC $ y(0) = 0, y'(0) = 0, y''(0) = 41, y'''(0) = 0 $,
          \begin{align}
              0     & = c_{1} + c_{3} + c_{4}                        \\
              0     & = 4c_{2} - 5c_{3} + 5c_{4}                     \\
              41    & = -16c_{1} + 25c_{3} + 25c_{4}                 \\
              0     & = -64c_{2} - 125c_{3} + 125c_{4}               \\
              y_{h} & = \color{y_h} -\cos x + 0.5e^{-5x} + 0.5e^{5x}
          \end{align}
          \begin{figure}[H]
              \centering
              \begin{tikzpicture}[
                      declare function = {
                              y_p = -cos(4*x) + cosh(5*x) ;
                          }
                  ]
                  \begin{axis}[
                          domain = -0.4:0.4,
                          legend pos = south west,
                          grid = both,
                          Ani,
                      ]
                      \addplot[GraphSmooth, y_p]{y_p};
                      \addlegendentry{$y_{p}$};
                  \end{axis}
              \end{tikzpicture}
          \end{figure}

    \item Solving the h-ODE,
          \begin{align}
              0               & = y^{v} - 5y''' + 4y'                            \\
              0               & = \lambda^{5} - 5\lambda^{3} + 4\lambda          \\
              \{\lambda_{i}\} & = \{-2, -1, 0, 1, 2\}                            \\
              y_{h}           & = \color{y_h} c_{1}e^{-2x} + c_{2}e^{-x} + c_{3}
              + c_{4}e^{x} + c_{5}e^{2x}
          \end{align}
          Applying IC $ y(0) = 0, y'(0) = -5, y''(0) = 11, y'''(0) = -23,
              y^{iv}(0) = 47 $,
          \begin{align}
              0     & = c_{1} + c_{2} + c_{3} + c_{4} + c_{5} \\
              -5    & = -2c_{1} - c_{2} + c_{4} + 2c_{5}      \\
              11    & = 4c_{1} + c_{2} + c_{4} + 4c_{5}       \\
              -23   & = -8c_{1} - c_{2} + c_{4} + 8c_{5}      \\
              47    & = 16c_{1} + c_{2} + c_{4} + 16c_{5}     \\
              y_{h} & = \color{y_h} 3e^{-2x} - e^{-x} - 2
          \end{align}
          \begin{figure}[H]
              \centering
              \begin{tikzpicture}[
                      declare function = {
                              y_p = 3*e^(-2*x) - e^(-x) - 2;
                          }
                  ]
                  \begin{axis}[
                          domain = 0:5,
                          legend pos = south west,
                          grid = both,
                          Ani,
                      ]
                      \addplot[GraphSmooth, y_p]{y_p};
                      \addlegendentry{$y_{p}$};
                  \end{axis}
              \end{tikzpicture}
          \end{figure}

    \item Solving the h-ODE,
          \begin{align}
              0               & = y^{iv} + 0.45y''' - 0.165y'' + 0.0045y' - 0.00175y \\
              0               & = \lambda^{4} + 0.45\lambda^{3} - 0.165\lambda^{2}
              + 0.0045\lambda - 0.00175                                              \\
              \{\lambda_{i}\} & = \{-0.7, 0.25, -0.1i, 0.1i\}                        \\
              y_{h}           & = \color{y_h} c_{1}e^{-0.7x} + c_{2}e^{0.25x}
              + c_{3}\cos(0.1x) + c_{4}\sin(0.1x)
          \end{align}
          Applying IC $ y(0) = 17.4, y'(0) = -2.82, y''(0) = 2.0485, y'''(0)
              = -1.458675 $,
          \begin{align}
              17.4      & = c_{1} + c_{2} + c_{3}                                 \\
              -2.82     & = -0.7c_{1} + 0.25c_{2} + 0.1c_{4}                      \\
              2.0485    & = 0.49c_{1} + 0.0625c_{2} - 0.01c_{3}                   \\
              -1.458675 & = -0.343c_{1} + 0.015625c_{2} - 0.001c_{4}              \\
              y_{h}     & = \color{y_h} 4.3e^{-0.7x} + e^{0.25x} + 12.1\cos(0.1x)
              - 0.6\sin(0.1x)
          \end{align}
          \begin{figure}[H]
              \centering
              \begin{tikzpicture}[
                      declare function = {
                              y_p = 4.3*e^(-0.7*x) + e^(0.25*x)
                              + 12.1*cos(0.1*x) - 0.6*sin(0.1*x);
                          }
                  ]
                  \begin{axis}[
                          domain = 0:15,
                          legend pos = north west,
                          grid = both,
                          Ani,
                      ]
                      \addplot[GraphSmooth, y_p]{y_p};
                      \addlegendentry{$y_{p}$};
                  \end{axis}
              \end{tikzpicture}
          \end{figure}

    \item
          \begin{enumerate}
              \item For a constant coefficient ODE, if one solution $ \lambda_{1} $
                    is known,
                    \begin{align}
                        (\lambda - \lambda_{1}) \cdot h(\lambda) & = P(\lambda)
                    \end{align}
                    The remainder after factoring out $ (\lambda - \lambda_{1}) $ is also
                    a polynomial in $ \lambda $ corresponding to the ODE obtained after
                    reduction of order.
              \item $ y_{1} $ is a known solution of
                    \begin{align}
                        0                      & = y''' + p_{2}(x)y'' + p_{1}(x)y'
                        + p_{0}(x)y                                                   \\
                        \text{Let} \quad y_{2} & = uy_{1}                             \\
                        y_{2}'                 & = u'y_{1} + uy_{1}'                  \\
                        y_{2}''                & = u''y_{1} + uy_{1}'' + 2u'y_{1}'    \\
                        y_{2}'''               & = u'''y_{1} + 3u''y_{1}' + uy_{1}'''
                        + 3u'y_{1}''                                                  \\
                        0                      & = u'''[y_{1}] + u''[3y_{1}'
                        + p_{2}y_{1}]
                        + u'[3y_{1}'' + 2p_{2}y_{1}' + p_{1}y_{1}]  \nonumber         \\
                                               & + u[y_{1}''' + p_{2}y_{1}''
                        + p_{1}y_{1}'
                        + p_{0}y_{1}]
                    \end{align}
                    Setting $ z = u' $ and thus, $ u = \int z(x) \dl x $, the ODE of 1
                    lesser order is given by,
                    \begin{align}
                        y_{1}z'' + (3y_{1}' + p_{2}y_{1})z' + (3y_{1}'' + 2p_{2}y_{1}'
                        + p_{1}y_{1})z & = 0
                    \end{align}

              \item Applying the above method with $ y_{1} = x $,
                    \begin{align}
                        x^{3}y''' - 3x^{2}y'' + (6 - x^{2})xy' - (6 - x^{2})y
                                                               & = 0             \\
                        y_{2} = ux \qquad y_{2}'               & = u + xu'       \\
                        y_{2}'' =2u' + xu'' \qquad y_{2}'''    & = 3u'' + xu'''  \\
                        u'''[x^{4}] + u'[-x^{4}]               & = 0             \\
                        u''' - u'                              & = 0             \\
                        \text{Let} \quad u' = z \qquad z'' - z & = 0             \\
                        z                                      & = c_{1}e^{-x}
                        + c_{2}e^{x}                                             \\
                        u                                      & = c_{1}e^{-x}
                        + c_{2}e^{x}                                             \\
                        y_{2}                                  & = c_{1}\ xe^{x}
                        + c_{2}\ xe^{-x}
                    \end{align}

              \item TBC. Trying Euler Cauchy third order ODEs with a basis given by,
                    \begin{align}
                        \text{Basis}\ S         & = \{1, x, x^{2}\} \\
                        x^{2}y''' - 2xy'' + 2y' & = 0
                    \end{align}
                    By inspection, one of the solutions is $ x^{0} $. Reduction of order
                    is also trivial by assigning $ z = y' $.
                    \begin{align}
                        x^{2}z'' - 2xz' + 2z & = 0
                    \end{align}
                    This can be solved using the usual methods for Euler-Cauchy ODEs to
                    obtain $ x, x^{2} $ as the other two solutions to the oringinal ODE.
          \end{enumerate}

\end{enumerate}